PREFIX : <https://linked.data.gov.au/dataset/bdr/orgs/>
PREFIX cs: <https://linked.data.gov.au/dataset/bdr/orgs>
PREFIX schema: <https://schema.org/>
PREFIX skos: <http://www.w3.org/2004/02/skos/core#>
PREFIX xsd: <http://www.w3.org/2001/XMLSchema#>

# ACT
:ACTGOV 
    a 
        skos:Concept,
        schema:Organization ;
    schema:name "ACTGOV Wildlife Atlas" ;
    skos:definition "The Environment, Heritage and Parks division manages the authoritative ACT Wildlife Atlas database of plants and animal occurrence records, and other related biodiversity datasets, in the ACT."@en ;
    skos:historyNote "Defined by BDR admin as a real organisation, expected in data from Australian Capital Territory Government" ;
    skos:scopeNote "Custodian organisation for biodiversity data held by the Australian Capital Territory Government." ;
    skos:inScheme cs: ;
    skos:prefLabel "ACTGOV Wildlife Atlas"@en ;
    skos:altLabel "ACTGOV" ;
    skos:topConceptOf cs: ;
    schema:url "www.act.gov.au/environment"^^xsd:anyURI ;
    schema:parentOrganization :Environment-Heritage-and-Parks ;
    .

# ACT parent org
:Environment-Heritage-and-Parks 
    a 
        skos:concept,
        schema:Organization ;
    schema:name "Environment, Heritage and Parks" ;
    skos:historyNote "Defined by BDR admin as as a parent organisation for data from the Australian Capital Territory" ;
    skos:inScheme cs: ;
    skos:prefLabel "Environment, Heritage and Parks, ACT Government" ;
    schema:url "https://www.environment.act.gov.au"^^xsd:anyURI ;
    skos:topConceptOf cs: ;
    .

# Gaia Resources
:Gaia-Resources
    a 
        skos:concept,
        schema:Organization ;
    schema:name "Gaia Resources" ;
    schema:definition "Gaia Resources provide a range of services around technology consulting to organisations that work with the environment, or collecting organisations. We work with organisations that interact with the environment in a range of ways - strategy development, spatial analysis, spatial support, software development, support, data management, and training being a few of the services that we offer in this area."
    schema:scopeNote "Gaia Resources has been involved in developing the BDR data ingestion tool known as: Part-A. The tool takes incidental occurrence data and systematic survey data from csv templates and transforms it into Australian Biodiversity Information Standard formatted data in RDF for the BDR graph."
    skos:inScheme cs: ;
    skos:prefLabel "Gaia Resources" ;
    schema:url "https://www.gaiaresources.com.au/"^^xsd:anyURI ;
    skos:topConceptOf cs: ;
    .

# Qld
:QLD-WildNet 
    a 
        skos:Concept,
        schema:Organization ;
    schema:name "QLD WildNet" ;
    skos:definition "The WildNet platform contains curated occurrence records of priority species and is sourced from government research and monitoring, private and university research programs, business, natural resource management bodies and select citizen science programs. The platform supports Queensland’s biodiversity and protected areas by providing important wildlife information that underpins conservation policies, programs and management responses."@en ;
    skos:historyNote "Defined by BDR admin as a real organisation, expected in data from Queensland" ;
    skos:scopeNote "Biodiversity occurrence records approved for release to the BDR. Species represented are priority species in Queensland." ;
    skos:inScheme cs: ;
    skos:prefLabel "Queensland Government WildNet Wildlife Records"@en ;
    skos:topConceptOf cs: ;
    schema:url "https://www.qld.gov.au/environment/plants-animals/species-information/wildnet"^^xsd:anyURI ;
    schema:parentOrganization :Queensland-Department-of-the-Environment-Tourism-Science-and-Innovation ;
    .

# Qld parent org
:Queensland-Department-of-the-Environment-Tourism-Science-and-Innovation 
    a 
        skos:concept,
        schema:Organization ;
    schema:name "Queensland Department of the Environment, Tourism, Science and Innovation" ;
    skos:historyNote "Defined by BDR admin as as a parent organisation for data from Queensland" ;
    skos:inScheme cs: ;
    skos:prefLabel "Queensland Department of the Environment, Tourism, Science and Innovation" ;
    schema:url "https://www.detsi.qld.gov.au/"^^xsd:anyURI ;
    skos:topConceptOf cs: ;
    schema:successorOf <https://linked.data.gov.au/org/des> ;
    .

# NSW
:NSW-BioNet 
    a 
        skos:Concept,
        schema:Organization ;
    schema:name "NSW BioNet" ;
    skos:definition "BioNet is the repository for biodiversity data products managed by the Department of Climate Change, Energy, the Environment and Water. BioNet aims to improve biodiversity outcomes by enabling the community and government to proactively manage and enhance biodiversity in New South Wales through comprehensive, credible and robust data and information. BioNet delivers two of its data collections to BDR: BioNet Species Sightings Data Collection and BioNet Systematic Survey Data Collection."@en ;
    skos:historyNote "Defined by BDR admin as a real organisation, expected in data from New South Wales" ;
    skos:scopeNote "Custodian organisation for biodiversity data held by the New South Wales Government." ;
    skos:inScheme cs: ;
    skos:prefLabel "BioNet Atlas of NSW Wildlife"@en ;
    skos:topConceptOf cs: ;
    schema:url "https://www.environment.nsw.gov.au/topics/animals-and-plants/biodiversity/nsw-bionet"^^xsd:anyURI ;
    schema:parentOrganization :Department-of-Climate-Change-Energy-and-the-Environment-NSW ;
    .

# NSW parent organisation
:Department-of-Climate-Change-Energy-and-the-Environment-NSW
    a 
        skos:concept,
        schema:Organization ;
    schema:name "Department of Climate Change Energy and the Environment - NSW" ;
    skos:historyNote "Defined by BDR admin as as a parent organisation for data from New South Wales" ;
    skos:inScheme cs: ;
    skos:prefLabel "Department of Climate Change Energy and the Environment - NSW" ;
    schema:url "https://www.nsw.gov.au/departments-and-agencies/dcceew"^^xsd:anyURI ;
    skos:topConceptOf cs: ;
    .

# NT
:NT-Atlas 
    a 
        skos:Concept,
        schema:Organization ;
    schema:name "NT Atlas" .
    skos:definition "Provider of NR Maps (Natural Resource Maps)"@en ;
    skos:historyNote "Defined by BDR admin as a real organisation, expected in data from the Northern Territory" ;
    skos:scopeNote "Custodian organisation for biodiversity data held by the Northern Territory Government." ;
    skos:inScheme cs: ;
    skos:prefLabel "NT Atlas"@en ;
    skos:altLabel "NT Flora Atlas",
        "NT Fauna Atlas", 
        "NR Maps" ;
    skos:topConceptOf cs: ;
    schema:url "https://nrmaps.nt.gov.au/biodiversity.html"^^xsd:anyURI ;
    schema:parentOrganization :Department-of-Lands-Planning-and-Environment ;
    .

# NT parent organisation
:Department-of-Lands-Planning-and-Environment
    a 
        skos:concept,
        schema:Organization ;
    schema:name "Department of Lands, Planning and Environment" ;
    skos:historyNote "Defined by BDR admin as as a parent organisation for data from the Northern Territory" ;
    skos:inScheme cs: ;
    skos:prefLabel "Department of Lands, Planning and Environment" ;
    schema:url "https://environment.nt.gov.au/"^^xsd:anyURI ;
    skos:altLabel "DLPE" ;
    skos:topConceptOf cs: ;
    .

# SA
:BDBSA
    a 
        skos:Concept,
        schema:Organization ;
    schema:name "Biological Databases of South Australia" ;
    skos:definition "Provider of the Biological Databases of South Australia (BDBSA). The BDBSA is South Australia's flora and fauna database that stores and manages survey and observation records, as well as taxonomic systems. This vital resource is critical to support decision-making processes for environmental issues within South Australian and Australian governments, as well as the wider community interested in biodiversity conservation."@en ;
    skos:historyNote "Defined by BDR admin as a real organisation, expected in data from South Australia" ;
    skos:scopeNote "Core repository for biodiversity data held by the South Australian Government." ;
    skos:inScheme cs: ;
    skos:prefLabel "Biological Databases of South Australia"@en ;
    skos:altLabel "BDBSA" ;
    skos:closeMatch <https://linked.data.gov.au/dataset/bdbsa> ;
    skos:topConceptOf cs: ;
    schema:url "https://www.environment.sa.gov.au/topics/science/information-and-data/biological-databases-of-south-australia"^^xsd:anyURI ;
    schema:parentOrganization <https://linked.data.gov.au/org/dew> ;
    .

# TAS
:Tasmanian-Natural-Values-Atlas
    a 
        skos:Concept,
        schema:Organization ;
    schema:name "Tasmanian Natural Values Atlas" ;
    skos:definition "The Natural Values Atlas provides authoritative and comprehensive information on Tasmania's natural values. It draws together, in one centralised location, data on Tasmanian flora and fauna including threatened species and weeds, as well as Tasmanian geodiversity and soil survey data. It also incorporates access to other essential data sets such as TASVEG and Threatened Native Vegetation Communities maps. The Natural Values Atlas allows observations of plants and animals from various sources to be viewed, recorded and analysed. It can be used to search for information on plant and animal species from Tasmania, Australia and can display maps showing their location and extent. The observations of plants and animals recorded in the Natural Values Atlas have been collected by a variety of custodians through general species surveys and projects undertaken for scientific research, environmental assessments, and other purposes throughout the State since the 1800's. The Natural Values Atlas provides data products such as the Natural Values Report, which brings several data sets together providing a resource that can be used for desktop assessments of natural values for specific areas."@en ;
    skos:historyNote "Defined by BDR admin as a real organisation, expected in data from Tasmania" ;
    skos:scopeNote "Core repository for biodiversity data held by the Tasmanian Government." ;
    skos:inScheme cs: ;
    skos:prefLabel "Tasmanian Natural Values Atlas"@en ;
    skos:altLabel "NVA" ;
    skos:topConceptOf cs: ;
    schema:url "https://www.naturalvaluesatlas.tas.gov.au/"^^xsd:anyURI ;
    schema:parentOrganization :Department-of-Natural-Resources-and-Environment-Tasmania ;
    .

# TAS parent organisation
:Department-of-Natural-Resources-and-Environment-Tasmania
    a 
        skos:concept,
        schema:Organization ;
    schema:name "Department of Natural Resources and Environment Tasmania" ;
    skos:historyNote "Defined by BDR admin as as a parent organisation for data from Tasmania" ;
    skos:inScheme cs: ;
    skos:prefLabel "Department of Natural Resources and Environment Tasmania" ;
    skos:altLabel "NRE" ;
    schema:url "https://nre.tas.gov.au/"^^xsd:anyURI ;
    skos:topConceptOf cs: ;
    .

# VIC
:Victorian-Biodiversity-Atlas 
    a 
        skos:Concept,
        schema:Organization ;
    schema:name "Victorian Biodiversity Atlas" ;
    skos:definition "Provider of the Victorian Biodiverity Atlas. The VBA species observations are a foundation dataset that feeds into some of the many biodiversity tools used in everyday decision making - showing where wildlife is now and how this has changed over time.  This makes it a core input to the majority of the governments processes and programs that impact native species. "@en ;
    skos:historyNote "Defined by BDR admin as a real organisation, expected in data from Victoria" ;
    skos:scopeNote "Custodian organisation for biodiversity data held by the Victorian Government." ;
    skos:inScheme cs: ;
    skos:prefLabel "Victorian Biodiversity Atlas"@en ;
    skos:altLabel "VBA" ;
    skos:topConceptOf cs: ;
    schema:url "https://www.environment.vic.gov.au/biodiversity/victorian-biodiversity-atlas"^^xsd:anyURI ;
    schema:parentOrganization :Department-of-Energy-Environment-and-Climate-Action ;
    .
# VIC parent organisation
:Department-of-Energy-Environment-and-Climate-Action
    a 
        skos:concept,
        schema:Organization ;
    schema:name "Department of Energy, Environment and Climate Action - Victoria" ;
    skos:historyNote "Defined by BDR admin as as a parent organisation for data from Victoria" ;
    skos:inScheme cs: ;
    skos:prefLabel "Department of Energy, Environment and Climate Action - Victoria" ;
    skos:altLabel "DEECA" ;
    schema:url "https://www.deeca.vic.gov.au/"^^xsd:anyURI ;
    skos:topConceptOf cs: ;
    .

# WA
:Biodiversity-Information-Office 
    a 
        skos:Concept,
        schema:Organization ;
    schema:name "Biodiversity Information Office" ;
    skos:definition "The Biodiversity Information Office provides the Dandjoo platform. Dandjoo is Western Australia’s first whole-of-state biodiversity data platform, providing a way to discover and explore data from government, industry, and research providers."@en ;
    skos:historyNote "Defined by BDR admin as a real organisation, expected in data from Western Australia" ;
    skos:scopeNote "Custodian organisation for data sourced from within Western Australian environment-related sectors, including government, industry, research, and the community." ;
    skos:inScheme cs: ;
    skos:prefLabel "WA Biodiversity Information Office"@en ;
    skos:altLabel "WA BIO, Dandjoo" ;
    skos:topConceptOf cs: ;
    schema:url "https://bio.wa.gov.au/"^^xsd:anyURI ;
    schema:parentOrganization :Department-of-Biodiversity-Conservation-and-Attractions ;
    .
# WA parent organisation
:Department-of-Biodiversity-Conservation-and-Attractions
    a 
        skos:concept,
        schema:Organization ;
    schema:name "Department of Biodiversity, Conservation and Attractions" ;
    skos:historyNote "Defined by BDR admin as as a parent organisation for data from Western Australia" ;
    skos:inScheme cs: ;
    skos:prefLabel "Department of Biodiversity, Conservation and Attractions" ;
    skos:altLabel "DBCA" ;
    schema:url "https://www.dbca.wa.gov.au/"^^xsd:anyURI ;
    skos:topConceptOf cs: ;
    .

cs:
    a skos:ConceptScheme ;
    skos:definition "Known organisations that submit data to the Biodiversity Date Repository"@en ;
    skos:hasTopConcept
        :wamuseum ,
        <https://linked.data.gov.au/org/dcceew> ;
    skos:historyNote "This vocabulary was developed for the Biodiversity Data Repository and is live in that it grows with new data submissions from new organisations" ;
    skos:prefLabel "BDR Submitting Organisations"@en ;
    schema:creator <https://linked.data.gov.au/org/dcceew> ;
    schema:dateCreated "2024-07-09"^^xsd:date ;
    schema:dateModified "2024-07-10"^^xsd:date ;
    schema:license <http://purl.org/NET/rdflicense/cc-by4.0> ;
    schema:publisher <https://linked.data.gov.au/org/dcceew> ;
.